Isabroom.thy
@@ -3,9 +3,27 @@ theory Isabroom
 begin
 
 typedecl binop
+axiomatization apply_binop :: "binop \<Rightarrow> val \<Rightarrow> val \<Rightarrow> val"
 typedecl unop
+axiomatization apply_unop :: "unop \<Rightarrow> val \<Rightarrow> val"
 datatype condition = Eq | Neq | Leq | Le | Geq | Gr
-type_synonym 'a func = "string \<times> nat \<times> 'a option"
+
+fun eval_cond_aux :: "val \<Rightarrow> val \<Rightarrow> (byte \<Rightarrow> byte \<Rightarrow> bool) \<Rightarrow> bool \<Rightarrow> bool" where
+  "eval_cond_aux [] [] _ b = b"
+| "eval_cond_aux [] _ _ _ = undefined"
+| "eval_cond_aux _ [] _ _ = undefined"
+| "eval_cond_aux (v1#xs) (v2#ys) c b = (if v1=v2 then eval_cond_aux xs ys c b
+    else c v1 v2)"
+
+fun eval_cond :: "condition \<Rightarrow> val \<Rightarrow> val \<Rightarrow> bool" where
+  "eval_cond Eq v1 v2 = (v1=v2)"
+| "eval_cond Neq v1 v2 = (v1\<noteq>v2)"
+| "eval_cond Leq v1 v2 = eval_cond_aux v1 v2 (\<le>) True"
+| "eval_cond Le v1 v2 = eval_cond_aux v1 v2 (<) False"
+| "eval_cond Geq v1 v2 = eval_cond_aux v1 v2 (\<ge>) True"
+| "eval_cond Gr v1 v2 = eval_cond_aux v1 v2 (>) False"
+
+type_synonym 'a func = "string \<times> var list \<times> 'a option"
 
 datatype 'a command =
   AssignConst var val 
@@ -14,10 +32,10 @@ datatype 'a command =
 | Store var var
 | Malloc var var
 | Free var
-| BinOp binop var var
-| UnOp unop var
-| PtrPlus var var
-| PtrSub var var
+| BinOp binop var var var
+| UnOp unop var var
+| PtrPlus var var var
+| PtrSub var var var
 | Memcpy (dest: var) (source: var) (number: var)
 | Assume condition var var
 | Assert condition var var
@@ -39,9 +57,11 @@ abbreviation can_allocate_from :: "blocks \<Rightarrow> loc \<Rightarrow> blockn
     (\<forall>b\<in>set (raw_blocks B). \<not>(overlaps_with (n,l,l + (loc64_ops.from_val z)) b)) \<and>
     (\<forall>b\<in>set (raw_blocks B). (case b of (n',_,_) \<Rightarrow> n'\<noteq>n)) \<comment> \<open>The name is new and unique\<close>"
 
-inductive semantics :: "pre_config \<Rightarrow> 'a command \<Rightarrow> pre_config option \<Rightarrow> bool" where
-  "fits k x \<Longrightarrow> semantics (S,B,M) (AssignConst x k) (Some (Stack ((lookup S)(x:=k)),B,M))"
-| "size x = size y \<Longrightarrow> semantics (S,B,M) (AssignVar x y) (Some (Stack ((lookup S)(x:=lookup S y)),B,M))"
+context fixes cfg_lookup :: "string \<Rightarrow> pre_config \<Rightarrow> pre_config \<Rightarrow> bool" begin
+inductive semantics :: "pre_config \<Rightarrow> 'a command \<Rightarrow> pre_config option \<Rightarrow> bool"
+  where
+  "fits k x \<Longrightarrow> semantics (S,B,M) (AssignConst x k) (Some (update_stack S x k,B,M))"
+| "size x = size y \<Longrightarrow> semantics (S,B,M) (AssignVar x y) (Some (update_stack S x (lookup S y),B,M))"
 | LoadFail: 
   "\<comment> \<open>y does not point into any block, i.e. is an invalid location\<close>
   base B (loc64_ops.from_val (lookup S y)) = 0 \<or>
@@ -55,7 +75,7 @@ inductive semantics :: "pre_config \<Rightarrow> 'a command \<Rightarrow> pre_co
   (loc64_ops.from_val (lookup S y)) + (sizev x) \<le> (loc64_ops.from_val (lookup S y))));
   \<comment> \<open>The addressed memory cells are actually allocated.\<close>
   access M (loc64_ops.from_val (lookup S y)) (size x) = Some v\<rbrakk> \<Longrightarrow> 
-    semantics (S,B,M) (Load x y) (Some (Stack ((lookup S)(x:=v)), B, M))"
+    semantics (S,B,M) (Load x y) (Some (update_stack S x v, B, M))"
 | StoreFail:
   "\<comment> \<open>x does not point into any block, i.e. is an invalid location\<close>
   base B (loc64_ops.from_val (lookup S x)) = 0 \<or>
@@ -73,13 +93,80 @@ inductive semantics :: "pre_config \<Rightarrow> 'a command \<Rightarrow> pre_co
   (\<forall>v\<in>set (lookup S z). v = 0) \<or> (size x \<noteq> loc_N_B) \<Longrightarrow> 
   semantics (S,_,_) (Malloc x z) None"
 | MallocSuccessNull: "\<lbrakk>\<exists>v\<in>set (lookup S z). v \<noteq> 0; size x = loc_N_B\<rbrakk> \<Longrightarrow>
-  semantics (S,B,M) (Malloc x z) (Some (Stack ((lookup S)(x:=null x)),B,M))"
+  semantics (S,B,M) (Malloc x z) (Some (update_stack S x (null x),B,M))"
 | MallocSuccess: "\<lbrakk>\<exists>v\<in>set (lookup S z). v \<noteq> 0; size x = loc_N_B;
   \<comment> \<open>l and n are new, k is arbitrary\<close>
   can_allocate_from B l n (lookup S z); length k = length (lookup S z)\<rbrakk> \<Longrightarrow>
   semantics (S,B,M) (Malloc x z) 
-    (Some (Stack ((lookup S)(x:=loc64_ops.to_val l)), 
+    (Some (update_stack S  x (loc64_ops.to_val l), 
     Blocks ((n,l,l+(loc64_ops.from_val (lookup S z)))#raw_blocks B),
     update_memory M l k))"
+| FreeError: "loc64_ops.from_val (lookup S x) \<noteq> base B (loc64_ops.from_val (lookup S x))
+  \<Longrightarrow> semantics (S,B,_) (Free x) None"
+| FreeSuccess: "\<lbrakk>loc64_ops.from_val (lookup S x) = y; y = base B y\<rbrakk>
+  \<Longrightarrow> semantics (S,B,M) (Free x) (Some (S,free_block B y, free_memory M y (ende B y)))"
+| "semantics (S,B,M) (BinOp b x y z) 
+  (Some (update_stack S x (apply_binop b (lookup S y) (lookup S z)),B,M))"
+| "semantics (S,B,M) (UnOp u x y) 
+  (Some (update_stack S x (apply_unop u (lookup S y)),B,M))"
+| PtrPlusError: "\<lbrakk>y'=loc64_ops.from_val (lookup S y); z'=loc64_ops.from_val (lookup S z);
+  (\<forall>v\<in>set (lookup S y). v = 0) \<or> (y' + z' < base B y') \<or> (y' + z' > ende B y')\<rbrakk>
+  \<Longrightarrow> semantics (S,B,M) (PtrPlus _ y z) None"
+| PtrPlusSuccess: "\<lbrakk>y'=loc64_ops.from_val (lookup S y); z'=loc64_ops.from_val (lookup S z);
+  \<exists>v\<in>set (lookup S y). v \<noteq> 0; y' + z' \<ge> base B y'; y' + z' \<le> ende B y'\<rbrakk>
+  \<Longrightarrow> semantics (S,B,M) (PtrPlus x y z) (Some (update_stack S x (loc64_ops.to_val (y'+z')),B,M))"
+| PtrSubError: "\<lbrakk>y'=loc64_ops.from_val (lookup S y); z'=loc64_ops.from_val (lookup S z);
+  (\<forall>v\<in>set (lookup S y). v = 0) \<or> (from_block y' B \<noteq> from_block z' B)\<rbrakk>
+  \<Longrightarrow> semantics (S,B,M) (PtrSub _ y z) None"
+| PtrSubSuccess: "\<lbrakk>y'=loc64_ops.from_val (lookup S y); z'=loc64_ops.from_val (lookup S z);
+  \<exists>v\<in>set (lookup S y). v \<noteq> 0; from_block y' B = from_block z' B\<rbrakk>
+  \<Longrightarrow> semantics (S,B,M) (PtrSub x y z) (Some (update_stack S x (loc64_ops.to_val (y'-z')),B,M))"
+| MemcpyError: "\<lbrakk>y'=loc64_ops.from_val (lookup S y); z'=loc64_ops.from_val (lookup S z);
+  x'=loc64_ops.from_val (lookup S x);
+  \<comment> \<open>x or y do not point into any block, i.e. is an invalid location\<close>
+  from_block x' B = None \<or> from_block y' B = None \<or>
+  \<comment> \<open>The size is too big, i.e. we would read/write out of bounds\<close>
+  x'+z' > ende B x' \<or> y'+z' > ende B y' \<or>
+  \<comment> \<open>The two memory portions (pointer+size) overlap\<close>
+  intv (x'+z') (bounds (raw_blocks B) y') \<or> intv (y'+z') (bounds (raw_blocks B) x')\<rbrakk> 
+  \<Longrightarrow> semantics (S,B,M) (Memcpy x y z) None"
+| MemcpySuccess: "\<lbrakk>y'=loc64_ops.from_val (lookup S y); z'=loc64_ops.from_val (lookup S z);
+  from_block x' B \<noteq> None; from_block y' B \<noteq> None; x'+z' \<le> ende B x'; y'+z' \<le> ende B y';
+  \<not>(intv (x'+z') (bounds (raw_blocks B) y')); \<not>(intv (y'+z') (bounds (raw_blocks B) x'));
+  access M y' (unat z') = Some v\<rbrakk>
+  \<Longrightarrow> semantics (S,B,M) (Memcpy x y z) (Some (S,B,update_memory M x' v))"
+| "eval_cond c (lookup S x) (lookup S y) \<Longrightarrow> semantics (S,B,M) (Assume c x y) (Some (S,B,M))"
+| AssertError: "\<not> eval_cond c (lookup S x) (lookup S y) \<Longrightarrow> semantics (S,B,M) (Assert c x y) None"
+| AssertSuccess: "eval_cond c (lookup S x) (lookup S y) \<Longrightarrow> semantics (S,B,M) (Assert c x y) (Some (S,B,M))"
+| "\<lbrakk>distinct args; length args = length params; list_all2 (\<lambda>a p. size a = size p) args params;
+  cfg_lookup f (Stack (bind_args_to_params (lookup S) params args),B,M) (S',B',M')\<rbrakk>
+  \<Longrightarrow> semantics (S,B,M) (Call (f,params,_) args) 
+    (Some (Stack (bind_args_to_params (lookup S') args params),B',M'))"
+
+abbreviation cfg_step :: "'a edge \<Rightarrow> pre_config \<Rightarrow> pre_config \<Rightarrow> bool" where
+  "cfg_step e pre post \<equiv> semantics pre (fst (snd e)) (Some post)"
+
+abbreviation cfg_step_find :: "'a edge set \<Rightarrow> CFG_node \<Rightarrow> CFG_node  \<Rightarrow> pre_config \<Rightarrow> pre_config \<Rightarrow> bool" where
+  "cfg_step_find es from to pre post \<equiv> \<exists>cmd. (from,cmd,to) \<in> es \<and> semantics pre cmd (Some post)"
+
+inductive cfg_reachable :: "'a edge set \<Rightarrow> CFG_node \<Rightarrow> CFG_node \<Rightarrow> pre_config \<Rightarrow> pre_config \<Rightarrow> bool" where
+  SingleStep: "cfg_step_find es from to pre post \<Longrightarrow> cfg_reachable es from to pre post"
+| MultiStep: "\<lbrakk>cfg_step_find es from to' pre interm; cfg_reachable es to' to interm post\<rbrakk>
+  \<Longrightarrow> cfg_reachable es from to pre post"
+
+abbreviation cfg_semantics :: "'a cfg \<Rightarrow> pre_config \<Rightarrow> pre_config \<Rightarrow> bool" where
+  "cfg_semantics cfg pre post \<equiv> cfg_reachable (snd cfg) entry exit pre post"
+end
+
+fun find_fun :: "(string \<rightharpoonup> 'a cfg) \<Rightarrow> string \<Rightarrow> pre_config \<Rightarrow> pre_config \<Rightarrow> bool" where
+  "find_fun funs f pre post = 
+    (case (funs f) of Some cfg \<Rightarrow> cfg_semantics (find_fun funs) cfg pre post
+    | None \<Rightarrow> False)"
+
+definition program_semantics :: "(string \<rightharpoonup> 'a cfg) \<Rightarrow> 'a cfg \<Rightarrow> pre_config \<Rightarrow> pre_config \<Rightarrow> bool" where
+  "program_semantics funs cfg pre post = 
+  cfg_semantics 
+    (\<lambda>name pre post. case (funs name) of Some cfg \<Rightarrow> cfg_semantics cfg pre post | None \<Rightarrow> False)
+  cfg pre post"
 
 end
